compile_inv & compile_inv_is_inv

compiler/src/Simulation.v
@@ -14,6 +14,32 @@ Definition simulation{State1 State2: Type}
     exec1 s1 post1 ->
     exec2 s2 (fun s2' => exists s1', related s1' s2' /\ post1 s1').
 
+Definition compile_inv{State1 State2: Type}
+           (related: State1 -> State2 -> Prop)(inv: State1 -> Prop): State2 -> Prop :=
+  fun s2 => exists s1, related s1 s2 /\ inv s1.
+
+(* More readable if inlined.
+   Note: only meaningful if exec is guaranteed to make progress.
+Definition is_inv{State: Type}(exec: State -> (State -> Prop) -> Prop)(inv: State -> Prop): Prop :=
+  forall s, inv s -> exec s inv.
+*)
+
+Lemma compile_inv_is_inv{State1 State2: Type}
+      (exec1: State1 -> (State1 -> Prop) -> Prop)
+      (exec2: State2 -> (State2 -> Prop) -> Prop)
+      (related: State1 -> State2 -> Prop)
+      (Sim: simulation exec1 exec2 related)
+      (inv1: State1 -> Prop)
+      (inv1_is_inv: forall s1, inv1 s1 -> exec1 s1 inv1):
+  forall s2, compile_inv related inv1 s2 -> exec2 s2 (compile_inv related inv1).
+Proof.
+  unfold compile_inv, simulation in *.
+  intros s2 (s1 & R & I1).
+  eapply Sim.
+  - exact R.
+  - eapply inv1_is_inv. exact I1.
+Qed.
+
 Definition compose_relation{State1 State2 State3: Type}
            (R12: State1 -> State2 -> Prop)(R23: State2 -> State3 -> Prop):
   State1 -> State3 -> Prop :=
